no message

execution/examples/Dexter2CPMM.v
@@ -22,6 +22,7 @@ From ConCert.Execution.Examples Require Import Common.
 From ConCert.Execution.Examples Require Import FA2Token.
 From ConCert.Execution.Examples Require Import FA2Interface.
 From ConCert.Execution.Examples Require Import Dexter2FA12.
+From ConCert.Execution.Examples Require Import InterContractCommunication.
 From ConCert.Execution.Examples Require Import SerializableUtil.
 From Coq Require Import ZArith.
 From Coq Require Import List.
@@ -525,7 +526,7 @@ Module DSInstances <: Dexter2Serializable.
                                             TokenToToken>.
 
     Global Instance Dexter2FA12_Msg_serialize `{ChainBase} : Serializable Dexter2FA12.Msg :=
-      msg_serializable.
+      Dexter2FA12.msg_serializable.
 
     Global Instance setup_serializable `{ChainBase} : Serializable Setup :=
       Derive Serializable Setup_rect <build_setup>.
@@ -2023,7 +2024,7 @@ Section Theories.
   Definition mintedOrBurnedTokens_acts (act_body : ActionBody) : Z :=
     match act_body with
     | act_call _ _ msg_serialized =>
-      match @deserialize Dexter2FA12.Msg msg_serializable msg_serialized with
+      match @deserialize Dexter2FA12.Msg Dexter2FA12.msg_serializable msg_serialized with
       | Some msg => mintedOrBurnedTokens (Some msg)
       | _ => 0
       end
@@ -2033,28 +2034,15 @@ Section Theories.
   Definition mintedOrBurnedTokens_tx (tx : Tx) : Z :=
     match tx.(tx_body) with
     | tx_call (Some msg_serialized) =>
-      match @deserialize Dexter2FA12.Msg msg_serializable msg_serialized with
+      match @deserialize Dexter2FA12.Msg Dexter2FA12.msg_serializable msg_serialized with
       | Some msg => mintedOrBurnedTokens (Some msg)
       | _ => 0
       end
     | _ => 0
     end.
 
-  Definition txCallTo (addr : Address) (tx : Tx) : bool :=
-    match tx.(tx_body) with
-    | tx_call _ => (tx.(tx_to) =? addr)%address
-    | _ => false
-    end.
-
-  Definition actTo (addr : Address) (act : ActionBody) : bool :=
-    match act with
-    | act_transfer to _ => (to =? addr)%address
-    | act_call to _ _ => (to =? addr)%address
-    | _ => false
-    end.
-
   Lemma deserialize_balance_of_ne_mint_or_burn : forall n m,
-    @deserialize Dexter2FA12.Msg msg_serializable (serialize (FA2Token.msg_balance_of n)) <>
+    @deserialize Dexter2FA12.Msg Dexter2FA12.msg_serializable (serialize (FA2Token.msg_balance_of n)) <>
     Some (Dexter2FA12.msg_mint_or_burn m).
   Proof.
     intros.
@@ -2077,7 +2065,7 @@ Section Theories.
           Forall (fun act_body =>
             match act_body with
             | act_call _ _ msg =>
-              match @deserialize Dexter2FA12.Msg msg_serializable msg with
+              match @deserialize Dexter2FA12.Msg Dexter2FA12.msg_serializable msg with
               | Some (msg_mint_or_burn _) => False
               | _ => True
               end
@@ -2242,7 +2230,7 @@ Section Theories.
         Forall (fun act_body =>
           match act_body with
           | act_call to _ msg_serialized =>
-            match @deserialize Dexter2FA12.Msg msg_serializable msg_serialized with
+            match @deserialize Dexter2FA12.Msg Dexter2FA12.msg_serializable msg_serialized with
             | Some (msg_mint_or_burn _) => to = lqtAddress cstate
             | _ => True
             end
@@ -2259,7 +2247,7 @@ Section Theories.
           Forall (fun act_body =>
             match act_body with
             | act_call _ _ msg =>
-              match @deserialize Dexter2FA12.Msg msg_serializable msg with
+              match @deserialize Dexter2FA12.Msg Dexter2FA12.msg_serializable msg with
               | Some (msg_mint_or_burn _) => False
               | _ => True
               end
@@ -2372,7 +2360,7 @@ Section Theories.
           Forall (fun tx =>
             match tx.(tx_body) with
             | tx_call (Some msg) =>
-              match @deserialize Dexter2FA12.Msg msg_serializable msg with
+              match @deserialize Dexter2FA12.Msg Dexter2FA12.msg_serializable msg with
               | Some (msg_mint_or_burn _) => False
               | _ => True
               end
@@ -2538,7 +2526,7 @@ Section Theories.
         Forall (fun tx =>
           match tx.(tx_body) with
           | tx_call (Some msg) =>
-            match @deserialize Dexter2FA12.Msg msg_serializable msg with
+            match @deserialize Dexter2FA12.Msg Dexter2FA12.msg_serializable msg with
             | Some (msg_mint_or_burn _) => tx.(tx_to) = lqtAddress cstate
             | _ => True
             end
@@ -2857,223 +2845,6 @@ Section Theories.
   Qed.
   Local Close Scope Z_scope.
 
-  Lemma deployed_incoming_calls_typed : forall bstate caddr {Setup Msg State : Type}
-            `{Serializable Setup}
-            `{Serializable Msg}
-            `{Serializable State}
-            {contract : Contract Setup Msg State}
-            (trace : ChainTrace empty_state bstate),
-    env_contracts bstate caddr = Some (contract : WeakContract) ->
-    exists inc_calls, 
-      incoming_calls Msg trace caddr = Some inc_calls.
-  Proof.
-    intros * deployed.
-    remember empty_state.
-    induction trace; eauto; subst.
-    destruct_chain_step; try destruct_action_eval; try rewrite_environment_equiv; auto.
-    - cbn in *.
-      destruct_address_eq; eauto.
-      now rewrite undeployed_contract_no_in_calls.
-    - cbn in *.
-      destruct IHtrace as [? IH]; auto.
-      rewrite IH.
-      clear IH.
-      destruct_address_eq; eauto.
-      subst.
-      rewrite deployed in deployed0.
-      inversion deployed0.
-      subst. clear deployed0.
-      apply wc_receive_strong in receive_some as
-        (prev_state' & msg' & new_state' & serialize_prev_state & msg_ser & serialize_new_state & receive_some).
-      cbn in receive_some.
-      destruct msg';
-        try rewrite msg_ser; eauto.
-      cbn in msg_ser.
-      destruct msg; eauto.
-      now rewrite msg_ser.
-    - now rewrite prev_next in *.
-  Qed.
-
-  Lemma undeployed_contract_no_state : forall bstate caddr (trace : ChainTrace empty_state bstate),
-    env_contracts bstate caddr = None ->
-    env_contract_states bstate caddr = None.
-  Proof.
-    intros * trace not_deployed.
-    remember empty_state.
-    induction trace; subst; auto.
-    destruct_chain_step; try destruct_action_eval;
-      try rewrite_environment_equiv; auto;
-      cbn in *;
-      try now destruct_address_eq;
-      try now rewrite prev_next in *.
-  Qed.
-
-  Lemma no_outgoing_txs_to_undeployed_contract : forall bstate caddr_main caddr_lqt (trace : ChainTrace empty_state bstate),
-    env_contracts bstate caddr_main = Some (contract : WeakContract) ->
-    env_contracts bstate caddr_lqt = None ->
-      filter (txCallTo caddr_lqt) (outgoing_txs trace caddr_main) = [].
-  Proof.
-    intros * deployed_main not_deployed_lqt.
-    remember empty_state.
-    induction trace; subst; try discriminate.
-    destruct_chain_step; try destruct_action_eval; try rewrite_environment_equiv; auto; cbn in *.
-    - now destruct_address_eq.
-    - destruct_address_eq; try easy; subst; cbn;
-        eapply undeployed_contract_no_out_txs in not_deployed; auto;
-        unfold outgoing_txs in not_deployed;
-        now rewrite not_deployed.
-    - destruct_address_eq; auto.
-      cbn.
-      now destruct_address_eq.
-    - now rewrite prev_next in *.
-  Qed.
-
-  Lemma no_incoming_calls_from_undeployed_contract : forall bstate caddr_main caddr_lqt (trace : ChainTrace empty_state bstate),
-    env_contracts bstate caddr_main = None ->
-    address_is_contract caddr_main = true ->
-    env_contracts bstate caddr_lqt = Some (Dexter2FA12.contract : WeakContract) ->
-    exists inc_calls,
-      incoming_calls Dexter2FA12.Msg trace caddr_lqt = Some inc_calls /\
-      filter (callFrom caddr_main) inc_calls = [].
-  Proof.
-    intros * not_deployed_main main_contract deployed_lqt.
-    remember empty_state.
-    induction trace; subst; try discriminate.
-    destruct_chain_step; try destruct_action_eval; try rewrite_environment_equiv; auto; cbn in *.
-    - destruct_address_eq; try easy; subst; cbn.
-      now rewrite undeployed_contract_no_in_calls by auto.
-    - destruct_address_eq; auto.
-      subst.
-      rewrite deployed_lqt in deployed.
-      inversion deployed.
-      subst. clear deployed.
-      apply wc_receive_strong in receive_some as
-        (prev_state' & msg' & new_state' & serialize_prev_state & msg_ser & serialize_new_state & receive_some).
-      cbn in receive_some.
-      destruct IHtrace as (? & calls & ?); auto.
-      apply undeployed_contract_no_out_queue in not_deployed_main; try easy.
-      rewrite queue_prev in not_deployed_main.
-      destruct msg';
-        [cbn in msg_ser; destruct msg; try easy|];
-        setoid_rewrite msg_ser;
-        rewrite calls;
-        eexists;
-        split; eauto;
-        unfold callFrom; cbn;
-        destruct_address_eq; auto;
-        subst;
-        apply Forall_inv in not_deployed_main;
-        now rewrite address_eq_refl in not_deployed_main.
-    - now rewrite prev_next in *.
-  Qed.
-
-  Definition contract_call_info_to_tx `{X : Type} `{Serializable X} (caddr : Address) (call_info : ContractCallInfo X) : Tx :=
-    let body :=
-      match call_info.(call_msg) with
-      | Some (msg) => tx_call (Some (serialize msg))
-      | None => tx_call None
-      end in
-    {|
-      tx_origin := call_info.(call_origin);
-      tx_from := call_info.(call_from);
-      tx_to := caddr;
-      tx_amount := call_info.(call_amount);
-      tx_body := body
-    |}.
-
-  Definition tx_to_contract_call_info `{X : Type} `{Serializable X} (tx : Tx) : option (ContractCallInfo X) :=
-    match tx.(tx_body) with
-    | tx_call None => Some
-      {|
-        call_origin := tx.(tx_origin);
-        call_from := tx.(tx_from);
-        call_amount := tx.(tx_amount);
-        call_msg := None
-      |}
-    | tx_call (Some m) => Some
-      {|
-        call_origin := tx.(tx_origin);
-        call_from := tx.(tx_from);
-        call_amount := tx.(tx_amount);
-        call_msg := @deserialize X _ m
-      |}
-    | _ => None
-    end.
-
-  Lemma incomming_eq_outgoing : forall bstate caddr_main caddr_lqt (trace : ChainTrace empty_state bstate),
-  (forall x (y : Dexter2FA12.Msg), deserialize x = Some y -> x = serialize y) ->
-    env_contracts bstate caddr_main = Some (contract : WeakContract) ->
-    env_contracts bstate caddr_lqt = Some (Dexter2FA12.contract : WeakContract) ->
-    exists inc_calls,
-      incoming_calls Dexter2FA12.Msg trace caddr_lqt = Some inc_calls /\
-      (filter (txCallTo caddr_lqt) (outgoing_txs trace caddr_main)) =
-      map (contract_call_info_to_tx caddr_lqt) (filter (callFrom caddr_main) inc_calls).
-  Proof.
-    intros * deserialize_right_inverse deployed_main deployed_lqt.
-    remember empty_state.
-    induction trace; subst; try discriminate.
-    destruct_chain_step; try destruct_action_eval; try rewrite_environment_equiv; auto.
-    - cbn in *.
-      destruct_address_eq; auto.
-    - cbn in *.
-      destruct_address_eq; auto; subst;
-        try (apply MCOption.some_inj in deployed_main; subst);
-        try (apply MCOption.some_inj in deployed_lqt; rewrite deployed_lqt in *; clear deployed_lqt);
-        try (rewrite undeployed_contract_no_in_calls by auto);
-        try (eapply undeployed_contract_no_out_txs in not_deployed as no_txs; eauto;
-              unfold outgoing_txs in no_txs; rewrite no_txs); cbn;
-        try (eapply no_outgoing_txs_to_undeployed_contract in not_deployed as no_txs; eauto;
-              unfold outgoing_txs in no_txs; rewrite no_txs);
-        try (eapply no_incoming_calls_from_undeployed_contract in not_deployed as (calls & inc_calls_eq & calls_eq); eauto;
-          exists calls; now rewrite inc_calls_eq, calls_eq);
-        try now exists [].
-    - cbn in *.
-      destruct_address_eq; subst; auto.
-      + rewrite deployed_lqt in deployed.
-        inversion deployed.
-        subst. clear deployed.
-        apply wc_receive_strong in receive_some as
-          (prev_state' & msg' & new_state' & serialize_prev_state & msg_ser & serialize_new_state & receive_some).
-        cbn in receive_some.
-        destruct IHtrace as (? & calls & IH); auto.
-        destruct msg' eqn:H;
-          [cbn in msg_ser; destruct msg eqn:H1; try easy|];
-          setoid_rewrite msg_ser;
-          rewrite calls;
-          eexists;
-          split; eauto.
-        * unfold callFrom in *; cbn.
-          rewrite !address_eq_refl.
-          cbn.
-          rewrite <- IH.
-          unfold contract_call_info_to_tx. cbn.
-          do 4 f_equal.
-          now apply deserialize_right_inverse.
-        * unfold callFrom in *; cbn.
-          rewrite !address_eq_refl.
-          cbn.
-          now rewrite <- IH.
-      + rewrite deployed_lqt in deployed.
-        inversion deployed.
-        subst. clear deployed.
-        apply wc_receive_strong in receive_some as
-          (prev_state' & msg' & new_state' & serialize_prev_state & msg_ser & serialize_new_state & receive_some).
-        cbn in receive_some.
-        destruct IHtrace as (? & calls & ?); auto.
-        destruct msg';
-          [cbn in msg_ser; destruct msg; try easy|];
-          setoid_rewrite msg_ser;
-          rewrite calls;
-          eexists;
-          split; eauto;
-          unfold callFrom; cbn;
-          now destruct_address_eq.
-      + cbn.
-        now rewrite address_eq_ne.
-    - cbn in *.
-      now rewrite prev_next in *.
-  Qed.
-
   Lemma mintedOrBurnedTokens_call_eq_tx : forall call_info addr,
     (fun callInfo => mintedOrBurnedTokens callInfo.(call_msg)) call_info =
     (fun callInfo => mintedOrBurnedTokens_tx (contract_call_info_to_tx addr callInfo)) call_info.
@@ -3134,8 +2905,10 @@ Section Theories.
     destruct main_correct as (state_main & depinfo_main & deployed_state_main & deploy_info_main & main_correct).
     apply (total_supply_correct _ _ trace) in deployed_lqt as lqt_correct.
     destruct lqt_correct as (state_lqt & depinfo_lqt & inc_calls_lqt & deployed_state_lqt & deploy_info_lqt & inc_acts_lqt & lqt_correct).
-    specialize (incomming_eq_outgoing) as (? & inc_acts_lqt' & calls_eq); eauto.
-    - intros. apply deserialize_lqt_token_msg_right_inverse; auto.
+    specialize incomming_eq_outgoing as incoming_eq.
+    edestruct incoming_eq as (? & inc_acts_lqt' & calls_eq);
+      [| apply deployed_main | apply deployed_lqt |].
+    - intros. eapply deserialize_lqt_token_msg_right_inverse; auto.
     - setoid_rewrite inc_acts_lqt in inc_acts_lqt'.
       inversion inc_acts_lqt'.
       subst. clear inc_acts_lqt'.
