execution/examples/InterContractCommunication.v
@@ -1,0 +1,260 @@
+From ConCert.Execution Require Import Blockchain.
+From ConCert.Execution Require Import Serializable.
+From Coq Require Import List.
+Import ListNotations.
+
+Section InterContractCommunication.
+Context {BaseTypes : ChainBase}.
+
+Definition txCallTo (addr : Address) (tx : Tx) : bool :=
+  match tx.(tx_body) with
+  | tx_call _ => (tx.(tx_to) =? addr)%address
+  | _ => false
+  end.
+
+Definition actTo (addr : Address) (act : ActionBody) : bool :=
+  match act with
+  | act_transfer to _ => (to =? addr)%address
+  | act_call to _ _ => (to =? addr)%address
+  | _ => false
+  end.
+
+Definition callFrom {Msg : Type} (addr : Address) (call_info : ContractCallInfo Msg) : bool :=
+  (call_info.(call_from) =? addr)%address.
+
+Lemma deployed_incoming_calls_typed : forall bstate caddr {Setup Msg State : Type}
+          `{Serializable Setup}
+          `{Serializable Msg}
+          `{Serializable State}
+          {contract : Contract Setup Msg State}
+          (trace : ChainTrace empty_state bstate),
+  env_contracts bstate caddr = Some (contract : WeakContract) ->
+  exists inc_calls, 
+    incoming_calls Msg trace caddr = Some inc_calls.
+Proof.
+  intros * deployed.
+  remember empty_state.
+  induction trace; eauto; subst.
+  destruct_chain_step; try destruct_action_eval; try rewrite_environment_equiv; auto.
+  - cbn in *.
+    destruct_address_eq; eauto.
+    now rewrite undeployed_contract_no_in_calls.
+  - cbn in *.
+    destruct IHtrace as [? IH]; auto.
+    rewrite IH.
+    clear IH.
+    destruct_address_eq; eauto.
+    subst.
+    rewrite deployed in deployed0.
+    inversion deployed0.
+    subst. clear deployed0.
+    apply wc_receive_strong in receive_some as
+      (prev_state' & msg' & new_state' & serialize_prev_state & msg_ser & serialize_new_state & receive_some).
+    cbn in receive_some.
+    destruct msg';
+      try rewrite msg_ser; eauto.
+    cbn in msg_ser.
+    destruct msg; eauto.
+    now rewrite msg_ser.
+  - now rewrite prev_next in *.
+Qed.
+
+Lemma undeployed_contract_no_state : forall bstate caddr (trace : ChainTrace empty_state bstate),
+  env_contracts bstate caddr = None ->
+  env_contract_states bstate caddr = None.
+Proof.
+  intros * trace not_deployed.
+  remember empty_state.
+  induction trace; subst; auto.
+  destruct_chain_step; try destruct_action_eval;
+    try rewrite_environment_equiv; auto;
+    cbn in *;
+    try now destruct_address_eq;
+    try now rewrite prev_next in *.
+Qed.
+
+Lemma no_outgoing_txs_to_undeployed_contract : forall bstate caddrA caddrB
+          (trace : ChainTrace empty_state bstate)
+          {Setup Msg State : Type}
+          `{Serializable Setup}
+          `{Serializable Msg}
+          `{Serializable State}
+          {contract : Contract Setup Msg State},
+  env_contracts bstate caddrA = Some (contract : WeakContract) ->
+  env_contracts bstate caddrB = None ->
+    filter (txCallTo caddrB) (outgoing_txs trace caddrA) = [].
+Proof.
+  intros * deployedA not_deployedB.
+  remember empty_state.
+  induction trace; subst; try discriminate.
+  destruct_chain_step; try destruct_action_eval; try rewrite_environment_equiv; auto; cbn in *.
+  - now destruct_address_eq.
+  - destruct_address_eq; try easy; subst; cbn;
+      eapply undeployed_contract_no_out_txs in not_deployed; auto;
+      unfold outgoing_txs in not_deployed;
+      now rewrite not_deployed.
+  - destruct_address_eq; auto.
+    cbn.
+    now destruct_address_eq.
+  - now rewrite prev_next in *.
+Qed.
+
+Lemma no_incoming_calls_from_undeployed_contract : forall bstate caddrA caddrB
+          (trace : ChainTrace empty_state bstate)
+          {Setup Msg State : Type}
+          `{Serializable Setup}
+          `{Serializable Msg}
+          `{Serializable State}
+          {contract : Contract Setup Msg State},
+  env_contracts bstate caddrA = None ->
+  address_is_contract caddrA = true ->
+  env_contracts bstate caddrB = Some (contract : WeakContract) ->
+  exists inc_calls,
+    incoming_calls Msg trace caddrB = Some inc_calls /\
+    filter (callFrom caddrA) inc_calls = [].
+Proof.
+  intros * not_deployedA A_is_contract deployedB.
+  remember empty_state.
+  induction trace; subst; try discriminate.
+  destruct_chain_step; try destruct_action_eval; try rewrite_environment_equiv; auto; cbn in *.
+  - destruct_address_eq; try easy; subst; cbn.
+    now rewrite undeployed_contract_no_in_calls by auto.
+  - destruct_address_eq; auto.
+    subst.
+    rewrite deployedB in deployed.
+    inversion deployed.
+    subst. clear deployed.
+    apply wc_receive_strong in receive_some as
+      (prev_state' & msg' & new_state' & serialize_prev_state & msg_ser & serialize_new_state & receive_some).
+    cbn in receive_some.
+    destruct IHtrace as (? & calls & ?); auto.
+    apply undeployed_contract_no_out_queue in not_deployedA; try easy.
+    rewrite queue_prev in not_deployedA.
+    destruct msg';
+      [cbn in msg_ser; destruct msg; try easy|];
+      setoid_rewrite msg_ser;
+      rewrite calls;
+      eexists;
+      split; eauto;
+      unfold callFrom; cbn;
+      destruct_address_eq; auto;
+      subst;
+      apply Forall_inv in not_deployedA;
+      now rewrite address_eq_refl in not_deployedA.
+  - now rewrite prev_next in *.
+Qed.
+
+Definition contract_call_info_to_tx `{X : Type} `{Serializable X} (caddr : Address) (call_info : ContractCallInfo X) : Tx :=
+  let body :=
+    match call_info.(call_msg) with
+    | Some (msg) => tx_call (Some (serialize msg))
+    | None => tx_call None
+    end in
+  {|
+    tx_origin := call_info.(call_origin);
+    tx_from := call_info.(call_from);
+    tx_to := caddr;
+    tx_amount := call_info.(call_amount);
+    tx_body := body
+  |}.
+
+Definition tx_to_contract_call_info `{X : Type} `{Serializable X} (tx : Tx) : option (ContractCallInfo X) :=
+  match tx.(tx_body) with
+  | tx_call None => Some
+    {|
+      call_origin := tx.(tx_origin);
+      call_from := tx.(tx_from);
+      call_amount := tx.(tx_amount);
+      call_msg := None
+    |}
+  | tx_call (Some m) => Some
+    {|
+      call_origin := tx.(tx_origin);
+      call_from := tx.(tx_from);
+      call_amount := tx.(tx_amount);
+      call_msg := @deserialize X _ m
+    |}
+  | _ => None
+  end.
+
+Lemma incomming_eq_outgoing : forall bstate caddrA caddrB
+          (trace : ChainTrace empty_state bstate)
+          {SetupA SetupB MsgA MsgB StateA StateB : Type}
+          `{Serializable SetupA} `{Serializable MsgA} `{Serializable StateA}
+          `{Serializable SetupB} `{Serializable MsgB} `{Serializable StateB}
+          {contractA : Contract SetupA MsgA StateA}
+          {contractB : Contract SetupB MsgB StateB},
+  (forall x (y : MsgB), deserialize x = Some y -> x = serialize y) ->
+  env_contracts bstate caddrA = Some (contractA : WeakContract) ->
+  env_contracts bstate caddrB = Some (contractB : WeakContract) ->
+  exists inc_calls,
+    incoming_calls MsgB trace caddrB = Some inc_calls /\
+    (filter (txCallTo caddrB) (outgoing_txs trace caddrA)) =
+    map (contract_call_info_to_tx caddrB) (filter (callFrom caddrA) inc_calls).
+Proof.
+  intros * deserialize_right_inverse deployedA deployedB.
+  remember empty_state.
+  induction trace; subst; try discriminate.
+  destruct_chain_step; try destruct_action_eval; try rewrite_environment_equiv; auto.
+  - cbn in *.
+    destruct_address_eq; auto.
+  - cbn in *.
+    destruct_address_eq; auto; subst;
+      try (apply MCOption.some_inj in deployedA; subst);
+      try (apply MCOption.some_inj in deployedB; rewrite deployedB in *; clear deployedB);
+      try (rewrite undeployed_contract_no_in_calls by auto);
+      try (eapply undeployed_contract_no_out_txs in not_deployed as no_txs; eauto;
+            unfold outgoing_txs in no_txs; rewrite no_txs); cbn;
+      try (eapply no_outgoing_txs_to_undeployed_contract in not_deployed as no_txs; cycle -1; eauto;
+            unfold outgoing_txs in no_txs; rewrite no_txs);
+      try (eapply no_incoming_calls_from_undeployed_contract in not_deployed; eauto;
+        destruct not_deployed as (calls & inc_calls_eq & calls_eq);
+        exists calls; now rewrite inc_calls_eq, calls_eq);
+      try now exists [].
+  - cbn in *.
+    destruct_address_eq; subst; auto.
+    + rewrite deployedB in deployed.
+      inversion deployed.
+      subst. clear deployed.
+      apply wc_receive_strong in receive_some as
+        (prev_state' & msg' & new_state' & serialize_prev_state & msg_ser & serialize_new_state & receive_some).
+      cbn in receive_some.
+      destruct IHtrace as (? & calls & IH); auto.
+      destruct msg';
+        [cbn in msg_ser; destruct msg; try easy|];
+        setoid_rewrite msg_ser;
+        rewrite calls;
+        eexists;
+        split; eauto.
+      * unfold callFrom in *; cbn.
+        rewrite !address_eq_refl.
+        cbn.
+        rewrite <- IH.
+        unfold contract_call_info_to_tx. cbn.
+        do 4 f_equal.
+        now apply deserialize_right_inverse.
+      * unfold callFrom in *; cbn.
+        rewrite !address_eq_refl.
+        cbn.
+        now rewrite <- IH.
+    + rewrite deployedB in deployed.
+      inversion deployed.
+      subst. clear deployed.
+      apply wc_receive_strong in receive_some as
+        (prev_state' & msg' & new_state' & serialize_prev_state & msg_ser & serialize_new_state & receive_some).
+      cbn in receive_some.
+      destruct IHtrace as (? & calls & ?); auto.
+      destruct msg';
+        [cbn in msg_ser; destruct msg; try easy|];
+        setoid_rewrite msg_ser;
+        rewrite calls;
+        eexists;
+        split; eauto;
+        unfold callFrom; cbn;
+        now destruct_address_eq.
+    + cbn.
+      now rewrite address_eq_ne.
+  - cbn in *.
+    now rewrite prev_next in *.
+Qed.
+End InterContractCommunication.
