execution/theories/Serializable.v
@@ -3,9 +3,9 @@ This format, SerializedValue, is either a unit/int/bool or a pair/list
 of these. We also define Serializable as a type class capturing that a
 type can be converted from and to this format. *)
 
-Require Import Monads.
-Require Import Containers.
-Require Import BoundedN.
+From ConCert.Execution Require Import Monads.
+From ConCert.Execution Require Import Containers.
+From ConCert.Execution Require Import BoundedN.
 From Coq Require Import Ascii.
 From Coq Require Import List.
 From Coq Require Import Psatz.
